src/spec/Flutterbye.Concurrency.Thread.fst
@@ -1,0 +1,34 @@
+// $legal:629:
+//
+// Copyright 2016 Michael Lowell Roberts & Microsoft Research
+//
+// Licensed under the Apache License, Version 2.0 (the "License");
+// you may not use this file except in compliance with the License.
+// You may obtain a copy of the License at
+//
+//     http://www.apache.org/licenses/LICENSE-2.0
+//
+// Unless required by applicable law or agreed to in writing, software
+// distributed under the License is distributed on an "AS IS" BASIS,
+// WITHOUT WARRANTIES OR CONDITIONS OF ANY KIND, either express or implied.
+// See the License for the specific language governing permissions and
+// limitations under the License.
+//
+//,$
+
+module Flutterbye.Concurrency.Thread
+open FStar.Seq
+open Flutterbye.Seq
+
+type step_t 'a =
+   | Commit: op:('a -> Tot 'a) -> step_t 'a
+   | Stale: op:('a -> Tot 'a) -> step_t 'a
+
+type thread_t 'a =
+   {
+      steps:seq (step_t 'a);
+      state:'a;
+   } 
+
+type is_something_committed_p (#a_t:Type) (steps:seq (step_t a_t)) =
+   satisfies_p is_Commit steps
